Renamings.

transformations/Moore2Mealy/Mealy.v
@@ -28,35 +28,35 @@ From core Require Import
 (* Base types *)
 
 
-Inductive State : Set :=
-  BuildState :
-  (* name *)  string ->
-  State.
+Record State : Set :=
+  BuildState 
+  { name :  string }.
 
-Inductive Transition : Set :=
-  BuildTransition :
-  (* input *)  string ->
-  (* output *)  string ->
-  Transition.
-
+Record Transition : Set :=
+  BuildTransition 
+  { input :  string ;
+    output :  string 
+  }.
 
 
-Inductive TransitionSource : Set :=
-   BuildTransitionSource :
-   Transition ->
-   State ->
-   TransitionSource.
+
+Record TransitionSource : Set :=
+   BuildTransitionSource 
+   { s_tr : Transition ;
+     s_st : State 
+   }.
 
 Definition maybeBuildTransitionSource (tr_arg: Transition) (so_arg: option (State)) : option TransitionSource :=
   match tr_arg, so_arg with
   | tr_arg_succ, Some so_arg_succ => Some (BuildTransitionSource tr_arg_succ so_arg_succ)
   | _, _ => None
   end.
-Inductive TransitionTarget : Set :=
-   BuildTransitionTarget :
-   Transition ->
-   State ->
-   TransitionTarget.
+
+Record TransitionTarget : Set :=
+  BuildTransitionTarget 
+    { t_tr : Transition ;
+      t_st : State 
+    }.
 
 Definition maybeBuildTransitionTarget (tr_arg: Transition) (ta_arg: option (State)) : option TransitionTarget :=
   match tr_arg, ta_arg with
@@ -67,95 +67,86 @@ Definition maybeBuildTransitionTarget (tr_arg: Transition) (ta_arg: option (Stat
 
 
 (* Accessors *)
-Definition State_getName (s : State) :  string :=
-  match s with BuildState  name  => name end.
-
-Definition Transition_getInput (t : Transition) :  string :=
-  match t with BuildTransition  input output  => input end.
-Definition Transition_getOutput (t : Transition) :  string :=
-  match t with BuildTransition  input output  => output end.
-
 
 Definition beq_State (st_arg1 : State) (st_arg2 : State) : bool :=
-(  beq_string (State_getName st_arg1) (State_getName st_arg2) )
-.
+  beq_string st_arg1.(name) st_arg2.(name).
 
 Definition beq_Transition (tr_arg1 : Transition) (tr_arg2 : Transition) : bool :=
-(  beq_string (Transition_getInput tr_arg1) (Transition_getInput tr_arg2) ) && 
-(  beq_string (Transition_getOutput tr_arg1) (Transition_getOutput tr_arg2) )
+(  beq_string tr_arg1.(input) tr_arg2.(input) ) && 
+(  beq_string tr_arg1.(output) tr_arg2.(output) )
 .
 
 
-(* Meta-types *)	
-Inductive MealyMetamodel_Class : Set :=
-  | StateClass
-  | TransitionClass
+(* Meta-types (kinds) *)	
+Inductive ElementKind : Set :=
+  | State_K
+  | Transition_K
 .
 
-Definition MealyMetamodel_getTypeByClass (mecl_arg : MealyMetamodel_Class) : Set :=
+Definition MealyMetamodel_getTypeByClass (mecl_arg : ElementKind) : Set :=
   match mecl_arg with
-    | StateClass => State
-    | TransitionClass => Transition
+    | State_K => State
+    | Transition_K => Transition
   end.	
 
-Inductive MealyMetamodel_Reference : Set :=
-| TransitionSourceReference
-| TransitionTargetReference
+Inductive LinkKind : Set :=
+  | TransitionSource_K
+  | TransitionTarget_K
 .
 
-Definition MealyMetamodel_getTypeByReference (mere_arg : MealyMetamodel_Reference) : Set :=
+Definition MealyMetamodel_getTypeByReference (mere_arg : LinkKind) : Set :=
   match mere_arg with
-| TransitionSourceReference => TransitionSource
-| TransitionTargetReference => TransitionTarget
+| TransitionSource_K => TransitionSource
+| TransitionTarget_K => TransitionTarget
   end.
 
-Definition MealyMetamodel_getERoleTypesByEReference (mere_arg : MealyMetamodel_Reference) : Set :=
+Definition MealyMetamodel_getERoleTypesByEReference (mere_arg : LinkKind) : Set :=
   match mere_arg with
-| TransitionSourceReference => (Transition * State)
-| TransitionTargetReference => (Transition * State)
+| TransitionSource_K => (Transition * State)
+| TransitionTarget_K => (Transition * State)
   end.
 
 (* Generic types *)			
 Inductive MealyMetamodel_Object : Set :=
  | Build_MealyMetamodel_Object : 
-    forall (mecl_arg: MealyMetamodel_Class), (MealyMetamodel_getTypeByClass mecl_arg) -> MealyMetamodel_Object.
+    forall (mecl_arg: ElementKind), (MealyMetamodel_getTypeByClass mecl_arg) -> MealyMetamodel_Object.
 
 Definition beq_MealyMetamodel_Object (c1 : MealyMetamodel_Object) (c2 : MealyMetamodel_Object) : bool :=
   match c1, c2 with
-  | Build_MealyMetamodel_Object StateClass o1, Build_MealyMetamodel_Object StateClass o2 => beq_State o1 o2
-  | Build_MealyMetamodel_Object TransitionClass o1, Build_MealyMetamodel_Object TransitionClass o2 => beq_Transition o1 o2
+  | Build_MealyMetamodel_Object State_K o1, Build_MealyMetamodel_Object State_K o2 => beq_State o1 o2
+  | Build_MealyMetamodel_Object Transition_K o1, Build_MealyMetamodel_Object Transition_K o2 => beq_Transition o1 o2
   | _, _ => false
   end.
 
 Inductive MealyMetamodel_Link : Set :=
  | Build_MealyMetamodel_Link : 
-    forall (mere_arg:MealyMetamodel_Reference), (MealyMetamodel_getTypeByReference mere_arg) -> MealyMetamodel_Link.
+    forall (mere_arg: LinkKind), (MealyMetamodel_getTypeByReference mere_arg) -> MealyMetamodel_Link.
 
 (* FIXME *)
 Definition beq_MealyMetamodel_Link (l1 : MealyMetamodel_Link) (l2 : MealyMetamodel_Link) : bool := true.
 
 (* Reflective functions *)
 Lemma MealyMetamodel_eqEClass_dec : 
- forall (mecl_arg1:MealyMetamodel_Class) (mecl_arg2:MealyMetamodel_Class), { mecl_arg1 = mecl_arg2 } + { mecl_arg1 <> mecl_arg2 }.
+ forall (mecl_arg1: ElementKind) (mecl_arg2: ElementKind), { mecl_arg1 = mecl_arg2 } + { mecl_arg1 <> mecl_arg2 }.
 Proof. repeat decide equality. Defined.
 
 Lemma MealyMetamodel_eqEReference_dec : 
- forall (mere_arg1:MealyMetamodel_Reference) (mere_arg2:MealyMetamodel_Reference), { mere_arg1 = mere_arg2 } + { mere_arg1 <> mere_arg2 }.
+ forall (mere_arg1: LinkKind) (mere_arg2: LinkKind), { mere_arg1 = mere_arg2 } + { mere_arg1 <> mere_arg2 }.
 Proof. repeat decide equality. Defined.
 
-Definition MealyMetamodel_getEClass (meob_arg : MealyMetamodel_Object) : MealyMetamodel_Class :=
+Definition MealyMetamodel_getEClass (meob_arg : MealyMetamodel_Object) : ElementKind :=
    match meob_arg with
   | (Build_MealyMetamodel_Object meob_arg _) => meob_arg
    end.
 
-Definition MealyMetamodel_getEReference (meli_arg : MealyMetamodel_Link) : MealyMetamodel_Reference :=
+Definition MealyMetamodel_getEReference (meli_arg : MealyMetamodel_Link) : LinkKind :=
    match meli_arg with
   | (Build_MealyMetamodel_Link meli_arg _) => meli_arg
    end.
 
 
 
-Definition MealyMetamodel_toClass (mecl_arg : MealyMetamodel_Class) (meob_arg : MealyMetamodel_Object) : option (MealyMetamodel_getTypeByClass mecl_arg).
+Definition MealyMetamodel_toClass (mecl_arg : ElementKind) (meob_arg : MealyMetamodel_Object) : option (MealyMetamodel_getTypeByClass mecl_arg).
 Proof.
   destruct meob_arg as [arg1 arg2].
   destruct (MealyMetamodel_eqEClass_dec arg1 mecl_arg) as [e|] eqn:dec_case.
@@ -164,7 +155,7 @@ Proof.
   - exact None.
 Defined.
 
-Definition MealyMetamodel_toReference (mere_arg : MealyMetamodel_Reference) (meli_arg : MealyMetamodel_Link) : option (MealyMetamodel_getTypeByReference mere_arg).
+Definition MealyMetamodel_toReference (mere_arg : LinkKind) (meli_arg : MealyMetamodel_Link) : option (MealyMetamodel_getTypeByReference mere_arg).
 Proof.
   destruct meli_arg as [arg1 arg2].
   destruct (MealyMetamodel_eqEReference_dec arg1 mere_arg) as [e|] eqn:dec_case.
@@ -187,10 +178,10 @@ Definition MealyMetamodel_Metamodel_Instance :
 
 Definition MealyModel := Model MealyMetamodel_Metamodel_Instance.
 
-Definition MealyMetamodel_toObject (mecl_arg: MealyMetamodel_Class) (t: MealyMetamodel_getTypeByClass mecl_arg) : MealyMetamodel_Object :=
+Definition MealyMetamodel_toObject (mecl_arg: ElementKind) (t: MealyMetamodel_getTypeByClass mecl_arg) : MealyMetamodel_Object :=
   (Build_MealyMetamodel_Object mecl_arg t).
 
-Definition MealyMetamodel_toLink (mere_arg: MealyMetamodel_Reference) (t: MealyMetamodel_getTypeByReference mere_arg) : MealyMetamodel_Link :=
+Definition MealyMetamodel_toLink (mere_arg: LinkKind) (t: MealyMetamodel_getTypeByReference mere_arg) : MealyMetamodel_Link :=
   (Build_MealyMetamodel_Link mere_arg t).
 
 
@@ -199,7 +190,7 @@ Definition MealyMetamodel_toLink (mere_arg: MealyMetamodel_Reference) (t: MealyM
 
 Fixpoint Transition_getSourceOnLinks (tr_arg : Transition) (l : list MealyMetamodel_Link) : option (State) :=
 match l with
-| (Build_MealyMetamodel_Link TransitionSourceReference (BuildTransitionSource Transition_ctr source_ctr)) :: l' => 
+| (Build_MealyMetamodel_Link TransitionSource_K (BuildTransitionSource Transition_ctr source_ctr)) :: l' => 
 	  if beq_Transition Transition_ctr tr_arg then Some source_ctr else Transition_getSourceOnLinks tr_arg l'
 | _ :: l' => Transition_getSourceOnLinks tr_arg l'
 | nil => None
@@ -210,12 +201,12 @@ Definition Transition_getSource (tr_arg : Transition) (m : MealyModel) : option 
   
 Definition Transition_getSourceObject (tr_arg : Transition) (m : MealyModel) : option (MealyMetamodel_Object) :=
   match Transition_getSource tr_arg m with
-  | Some st_arg => Some (MealyMetamodel_toObject StateClass st_arg) 
+  | Some st_arg => Some (MealyMetamodel_toObject State_K st_arg) 
   | _ => None
   end.
 Fixpoint Transition_getTargetOnLinks (tr_arg : Transition) (l : list MealyMetamodel_Link) : option (State) :=
 match l with
-| (Build_MealyMetamodel_Link TransitionTargetReference (BuildTransitionTarget Transition_ctr target_ctr)) :: l' => 
+| (Build_MealyMetamodel_Link TransitionTarget_K (BuildTransitionTarget Transition_ctr target_ctr)) :: l' => 
 	  if beq_Transition Transition_ctr tr_arg then Some target_ctr else Transition_getTargetOnLinks tr_arg l'
 | _ :: l' => Transition_getTargetOnLinks tr_arg l'
 | nil => None
@@ -226,7 +217,7 @@ Definition Transition_getTarget (tr_arg : Transition) (m : MealyModel) : option 
   
 Definition Transition_getTargetObject (tr_arg : Transition) (m : MealyModel) : option (MealyMetamodel_Object) :=
   match Transition_getTarget tr_arg m with
-  | Some st_arg => Some (MealyMetamodel_toObject StateClass st_arg) 
+  | Some st_arg => Some (MealyMetamodel_toObject State_K st_arg) 
   | _ => None
   end.
 
@@ -234,7 +225,7 @@ Definition Transition_getTargetObject (tr_arg : Transition) (m : MealyModel) : o
 (* Typeclass Instances *)	
 
 #[export]
-Instance MealyMetamodel_ElementDenotation : Denotation MealyMetamodel_Object MealyMetamodel_Class :=
+Instance MealyMetamodel_ElementDenotation : Denotation MealyMetamodel_Object ElementKind :=
 {
 	denoteDatatype := MealyMetamodel_getTypeByClass;
 	unbox := MealyMetamodel_toClass;
@@ -242,7 +233,7 @@ Instance MealyMetamodel_ElementDenotation : Denotation MealyMetamodel_Object Mea
 }.
 
 #[export]
-Instance MealyMetamodel_LinkDenotation : Denotation MealyMetamodel_Link MealyMetamodel_Reference :=
+Instance MealyMetamodel_LinkDenotation : Denotation MealyMetamodel_Link LinkKind :=
 {
 	denoteDatatype := MealyMetamodel_getTypeByReference;
 	unbox := MealyMetamodel_toReference;
@@ -262,7 +253,7 @@ Instance MealyMetamodel_ModelingMetamodel_Instance :
 (* Useful lemmas *)
 
 Lemma Mealy_invert : 
-  forall (mecl_arg: MealyMetamodel_Class) (t1 t2: MealyMetamodel_getTypeByClass mecl_arg), 
+  forall (mecl_arg: ElementKind) (t1 t2: MealyMetamodel_getTypeByClass mecl_arg), 
     Build_MealyMetamodel_Object mecl_arg t1 = Build_MealyMetamodel_Object mecl_arg t2 -> t1 = t2.
 Proof.
   intros ; Tactics.dep_inversion H ; assumption.
@@ -271,10 +262,10 @@ Qed.
 
 (* Not Used *)
 Definition MealyMetamodel_instanceOfEClass :
-  MealyMetamodel_Class -> MealyMetamodel_Object -> bool :=
+  ElementKind -> MealyMetamodel_Object -> bool :=
   MealyMetamodel_ElementDenotation.(instanceof).
 
 Definition MealyMetamodel_instanceOfEReference :
-  MealyMetamodel_Reference -> MealyMetamodel_Link -> bool :=
+  LinkKind -> MealyMetamodel_Link -> bool :=
   MealyMetamodel_LinkDenotation.(instanceof).
 
