transformations/Moore2Mealy/Moore.v
@@ -28,35 +28,34 @@ From core Require Import
 (* Base types *)
 
 
-Inductive State : Set :=
-  BuildState :
-  (* name *)  string ->
-  (* output *)  string ->
-  State.
+Record State : Set :=
+  BuildState 
+  {  name : string ;
+     output : string 
+  }.
 
-Inductive Transition : Set :=
-  BuildTransition :
-  (* input *)  string ->
-  Transition.
+Record Transition : Set :=
+  BuildTransition { input : string }.
 
 
 
-Inductive TransitionSource : Set :=
-   BuildTransitionSource :
-   Transition ->
-   State ->
-   TransitionSource.
+Record TransitionSource : Set :=
+  BuildTransitionSource 
+    { s_tr : Transition ;
+      s_st : State 
+    }.
 
 Definition maybeBuildTransitionSource (tr_arg: Transition) (so_arg: option (State)) : option TransitionSource :=
   match tr_arg, so_arg with
   | tr_arg_succ, Some so_arg_succ => Some (BuildTransitionSource tr_arg_succ so_arg_succ)
   | _, _ => None
   end.
-Inductive TransitionTarget : Set :=
-   BuildTransitionTarget :
-   Transition ->
-   State ->
-   TransitionTarget.
+
+Record TransitionTarget : Set :=
+   BuildTransitionTarget 
+   { t_tr : Transition ;
+     t_st : State 
+   }.
 
 Definition maybeBuildTransitionTarget (tr_arg: Transition) (ta_arg: option (State)) : option TransitionTarget :=
   match tr_arg, ta_arg with
@@ -67,95 +66,89 @@ Definition maybeBuildTransitionTarget (tr_arg: Transition) (ta_arg: option (Stat
 
 
 (* Accessors *)
-Definition State_getName (s : State) :  string :=
-  match s with BuildState  name output  => name end.
-Definition State_getOutput (s : State) :  string :=
-  match s with BuildState  name output  => output end.
 
-Definition Transition_getInput (t : Transition) :  string :=
-  match t with BuildTransition  input  => input end.
 
 
 Definition beq_State (st_arg1 : State) (st_arg2 : State) : bool :=
-(  beq_string (State_getName st_arg1) (State_getName st_arg2) ) && 
-(  beq_string (State_getOutput st_arg1) (State_getOutput st_arg2) )
+(  beq_string st_arg1.(name) st_arg2.(name) ) && 
+(  beq_string st_arg1.(output) st_arg2.(output) )
 .
 
 Definition beq_Transition (tr_arg1 : Transition) (tr_arg2 : Transition) : bool :=
-(  beq_string (Transition_getInput tr_arg1) (Transition_getInput tr_arg2) )
+(  beq_string tr_arg1.(input) tr_arg2.(input) )
 .
 
 
-(* Meta-types *)	
-Inductive MooreMetamodel_Class : Set :=
-  | StateClass
-  | TransitionClass
+(* Meta-types (or kinds, to be used in rules) *)	
+Inductive ElementKind : Set :=
+  | State_K
+  | Transition_K
 .
 
-Definition MooreMetamodel_getTypeByClass (mocl_arg : MooreMetamodel_Class) : Set :=
+Definition MooreMetamodel_getTypeByEKind (mocl_arg : ElementKind) : Set :=
   match mocl_arg with
-    | StateClass => State
-    | TransitionClass => Transition
+    | State_K => State
+    | Transition_K => Transition
   end.	
 
-Inductive MooreMetamodel_Reference : Set :=
-| TransitionSourceReference
-| TransitionTargetReference
+Inductive LinkKind : Set :=
+| TransitionSource_K
+| TransitionTarget_K
 .
 
-Definition MooreMetamodel_getTypeByReference (more_arg : MooreMetamodel_Reference) : Set :=
+Definition MooreMetamodel_getTypeByReference (more_arg : LinkKind) : Set :=
   match more_arg with
-| TransitionSourceReference => TransitionSource
-| TransitionTargetReference => TransitionTarget
+| TransitionSource_K => TransitionSource
+| TransitionTarget_K => TransitionTarget
   end.
 
-Definition MooreMetamodel_getERoleTypesByEReference (more_arg : MooreMetamodel_Reference) : Set :=
+Definition MooreMetamodel_getERoleTypesByEReference (more_arg : LinkKind) : Set :=
   match more_arg with
-| TransitionSourceReference => (Transition * State)
-| TransitionTargetReference => (Transition * State)
+| TransitionSource_K => (Transition * State)
+| TransitionTarget_K => (Transition * State)
   end.
 
 (* Generic types *)			
 Inductive MooreMetamodel_Object : Set :=
  | Build_MooreMetamodel_Object : 
-    forall (mocl_arg: MooreMetamodel_Class), (MooreMetamodel_getTypeByClass mocl_arg) -> MooreMetamodel_Object.
+    forall (mocl_arg: ElementKind), (MooreMetamodel_getTypeByEKind mocl_arg) -> MooreMetamodel_Object.
 
 Definition beq_MooreMetamodel_Object (c1 : MooreMetamodel_Object) (c2 : MooreMetamodel_Object) : bool :=
   match c1, c2 with
-  | Build_MooreMetamodel_Object StateClass o1, Build_MooreMetamodel_Object StateClass o2 => beq_State o1 o2
-  | Build_MooreMetamodel_Object TransitionClass o1, Build_MooreMetamodel_Object TransitionClass o2 => beq_Transition o1 o2
+  | Build_MooreMetamodel_Object State_K o1, Build_MooreMetamodel_Object State_K o2 => beq_State o1 o2
+  | Build_MooreMetamodel_Object Transition_K o1, Build_MooreMetamodel_Object Transition_K o2 => beq_Transition o1 o2
   | _, _ => false
   end.
 
 Inductive MooreMetamodel_Link : Set :=
  | Build_MooreMetamodel_Link : 
-    forall (more_arg:MooreMetamodel_Reference), (MooreMetamodel_getTypeByReference more_arg) -> MooreMetamodel_Link.
+    forall (more_arg: LinkKind), (MooreMetamodel_getTypeByReference more_arg) -> MooreMetamodel_Link.
 
 (* FIXME *)
 Definition beq_MooreMetamodel_Link (l1 : MooreMetamodel_Link) (l2 : MooreMetamodel_Link) : bool := true.
 
 (* Reflective functions *)
 Lemma MooreMetamodel_eqEClass_dec : 
- forall (mocl_arg1:MooreMetamodel_Class) (mocl_arg2:MooreMetamodel_Class), { mocl_arg1 = mocl_arg2 } + { mocl_arg1 <> mocl_arg2 }.
+ forall (mocl_arg1: ElementKind) (mocl_arg2: ElementKind), { mocl_arg1 = mocl_arg2 } + { mocl_arg1 <> mocl_arg2 }.
 Proof. repeat decide equality. Defined.
 
 Lemma MooreMetamodel_eqEReference_dec : 
- forall (more_arg1:MooreMetamodel_Reference) (more_arg2:MooreMetamodel_Reference), { more_arg1 = more_arg2 } + { more_arg1 <> more_arg2 }.
+ forall (more_arg1: LinkKind) (more_arg2: LinkKind), { more_arg1 = more_arg2 } + { more_arg1 <> more_arg2 }.
 Proof. repeat decide equality. Defined.
 
-Definition MooreMetamodel_getEClass (moob_arg : MooreMetamodel_Object) : MooreMetamodel_Class :=
+Definition MooreMetamodel_getEClass (moob_arg : MooreMetamodel_Object) : ElementKind :=
    match moob_arg with
   | (Build_MooreMetamodel_Object moob_arg _) => moob_arg
    end.
 
-Definition MooreMetamodel_getEReference (moli_arg : MooreMetamodel_Link) : MooreMetamodel_Reference :=
+Definition MooreMetamodel_getEReference (moli_arg : MooreMetamodel_Link) : LinkKind :=
    match moli_arg with
   | (Build_MooreMetamodel_Link moli_arg _) => moli_arg
    end.
 
 
 
-Definition MooreMetamodel_toClass (mocl_arg : MooreMetamodel_Class) (moob_arg : MooreMetamodel_Object) : option (MooreMetamodel_getTypeByClass mocl_arg).
+Definition MooreMetamodel_toClass (mocl_arg : ElementKind) (moob_arg : MooreMetamodel_Object) : option (MooreMetamodel_getTypeByEKind mocl_arg).
 Proof.
   destruct moob_arg as [arg1 arg2].
   destruct (MooreMetamodel_eqEClass_dec arg1 mocl_arg) as [e|] eqn:dec_case.
@@ -164,7 +157,7 @@ Proof.
   - exact None.
 Defined.
 
-Definition MooreMetamodel_toReference (more_arg : MooreMetamodel_Reference) (moli_arg : MooreMetamodel_Link) : option (MooreMetamodel_getTypeByReference more_arg).
+Definition MooreMetamodel_toReference (more_arg : LinkKind) (moli_arg : MooreMetamodel_Link) : option (MooreMetamodel_getTypeByReference more_arg).
 Proof.
   destruct moli_arg as [arg1 arg2].
   destruct (MooreMetamodel_eqEReference_dec arg1 more_arg) as [e|] eqn:dec_case.
@@ -187,10 +180,10 @@ Definition MooreMetamodel_Metamodel_Instance :
 
 Definition MooreModel := Model MooreMetamodel_Metamodel_Instance.
 
-Definition MooreMetamodel_toObject (mocl_arg: MooreMetamodel_Class) (t: MooreMetamodel_getTypeByClass mocl_arg) : MooreMetamodel_Object :=
+Definition MooreMetamodel_toObject (mocl_arg: ElementKind) (t: MooreMetamodel_getTypeByEKind mocl_arg) : MooreMetamodel_Object :=
   (Build_MooreMetamodel_Object mocl_arg t).
 
-Definition MooreMetamodel_toLink (more_arg: MooreMetamodel_Reference) (t: MooreMetamodel_getTypeByReference more_arg) : MooreMetamodel_Link :=
+Definition MooreMetamodel_toLink (more_arg: LinkKind) (t: MooreMetamodel_getTypeByReference more_arg) : MooreMetamodel_Link :=
   (Build_MooreMetamodel_Link more_arg t).
 
 
@@ -199,7 +192,7 @@ Definition MooreMetamodel_toLink (more_arg: MooreMetamodel_Reference) (t: MooreM
 
 Fixpoint Transition_getSourceOnLinks (tr_arg : Transition) (l : list MooreMetamodel_Link) : option (State) :=
 match l with
-| (Build_MooreMetamodel_Link TransitionSourceReference (BuildTransitionSource Transition_ctr source_ctr)) :: l' => 
+| (Build_MooreMetamodel_Link TransitionSource_K (BuildTransitionSource Transition_ctr source_ctr)) :: l' => 
 	  if beq_Transition Transition_ctr tr_arg then Some source_ctr else Transition_getSourceOnLinks tr_arg l'
 | _ :: l' => Transition_getSourceOnLinks tr_arg l'
 | nil => None
@@ -210,12 +203,12 @@ Definition Transition_getSource (tr_arg : Transition) (m : MooreModel) : option 
   
 Definition Transition_getSourceObject (tr_arg : Transition) (m : MooreModel) : option (MooreMetamodel_Object) :=
   match Transition_getSource tr_arg m with
-  | Some st_arg => Some (MooreMetamodel_toObject StateClass st_arg) 
+  | Some st_arg => Some (MooreMetamodel_toObject State_K st_arg) 
   | _ => None
   end.
 Fixpoint Transition_getTargetOnLinks (tr_arg : Transition) (l : list MooreMetamodel_Link) : option (State) :=
 match l with
-| (Build_MooreMetamodel_Link TransitionTargetReference (BuildTransitionTarget Transition_ctr target_ctr)) :: l' => 
+| (Build_MooreMetamodel_Link TransitionTarget_K (BuildTransitionTarget Transition_ctr target_ctr)) :: l' => 
 	  if beq_Transition Transition_ctr tr_arg then Some target_ctr else Transition_getTargetOnLinks tr_arg l'
 | _ :: l' => Transition_getTargetOnLinks tr_arg l'
 | nil => None
@@ -226,22 +219,22 @@ Definition Transition_getTarget (tr_arg : Transition) (m : MooreModel) : option 
   
 Definition Transition_getTargetObject (tr_arg : Transition) (m : MooreModel) : option (MooreMetamodel_Object) :=
   match Transition_getTarget tr_arg m with
-  | Some st_arg => Some (MooreMetamodel_toObject StateClass st_arg) 
+  | Some st_arg => Some (MooreMetamodel_toObject State_K st_arg) 
   | _ => None
   end.
 
 
 (* Typeclass Instances *)	
 #[export]
-Instance MooreMetamodel_ElementDenotation : Denotation MooreMetamodel_Object MooreMetamodel_Class :=
+Instance MooreMetamodel_ElementDenotation : Denotation MooreMetamodel_Object ElementKind :=
 {
-	denoteDatatype := MooreMetamodel_getTypeByClass;
+	denoteDatatype := MooreMetamodel_getTypeByEKind;
 	unbox := MooreMetamodel_toClass;
 	constructor := MooreMetamodel_toObject;
 }.
 
 #[export]
-Instance MooreMetamodel_LinkDenotation : Denotation MooreMetamodel_Link MooreMetamodel_Reference :=
+Instance MooreMetamodel_LinkDenotation : Denotation MooreMetamodel_Link LinkKind :=
 {
 	denoteDatatype := MooreMetamodel_getTypeByReference;
 	unbox := MooreMetamodel_toReference;
@@ -260,7 +253,7 @@ Instance MooreMetamodel_ModelingMetamodel_Instance :
 (* Useful lemmas *)
 
 Lemma Moore_invert : 
-  forall (mocl_arg: MooreMetamodel_Class) (t1 t2: MooreMetamodel_getTypeByClass mocl_arg), 
+  forall (mocl_arg: ElementKind) (t1 t2: MooreMetamodel_getTypeByEKind mocl_arg), 
     Build_MooreMetamodel_Object mocl_arg t1 = Build_MooreMetamodel_Object mocl_arg t2 -> t1 = t2.
 Proof.
   intros. Tactics.dep_inversion H. assumption.
@@ -268,10 +261,10 @@ Qed.
 
 (* Not Used *)
 Definition MooreMetamodel_instanceOfEClass :
-  MooreMetamodel_Class -> MooreMetamodel_Object -> bool :=
+  ElementKind -> MooreMetamodel_Object -> bool :=
   MooreMetamodel_ElementDenotation.(instanceof).
 
 Definition MooreMetamodel_instanceOfEReference :
-  MooreMetamodel_Reference -> MooreMetamodel_Link -> bool :=
+  LinkKind -> MooreMetamodel_Link -> bool :=
   MooreMetamodel_LinkDenotation.(instanceof).
 
