core/properties/injectivity/sampleMoore_injectivity.v
@@ -16,7 +16,7 @@
 Definition Moore_m1 : Model MooreMetamodel_Metamodel_Instance :=
 (Build_Model MooreMetamodel_Metamodel_Instance
     (
-        (Build_MooreMetamodel_Object StateClass (BuildState  "S0" "1")) :: nil
+        (Build_MooreMetamodel_Object State_K (BuildState  "S0" "1")) :: nil
     )
     (
         nil
@@ -26,7 +26,7 @@ Definition Moore_m1 : Model MooreMetamodel_Metamodel_Instance :=
 Definition Moore_m2 : Model MooreMetamodel_Metamodel_Instance :=
 (Build_Model MooreMetamodel_Metamodel_Instance
     (
-        (Build_MooreMetamodel_Object StateClass (BuildState  "S0" "0")) :: nil
+        (Build_MooreMetamodel_Object State_K (BuildState  "S0" "0")) :: nil
     )
     (
         nil
