transformations/Moore2Mealy/MooreSemantics.v
@@ -6,10 +6,10 @@ Require Import core.Model.
 Require Import core.utils.Utils.
 
 Definition MooreMetamodel_toStates (m: list MooreMetamodel_Object) : list State :=
-    optionList2List (map (fun s => (MooreMetamodel_toClass StateClass s)) m).
+    optionList2List (map (fun s => (MooreMetamodel_toClass State_K s)) m).
 
 Definition MooreMetamodel_toTransitions (m: list MooreMetamodel_Object) : list Transition :=
-    optionList2List (map (fun s => (MooreMetamodel_toClass TransitionClass s)) m).
+    optionList2List (map (fun s => (MooreMetamodel_toClass Transition_K s)) m).
 
 Definition MooreMetamodel_allStates (m: MooreModel) : list State :=
     MooreMetamodel_toStates m.(modelElements).
@@ -18,7 +18,7 @@ Definition MooreMetamodel_allTransitions (m: MooreModel) : list Transition :=
     MooreMetamodel_toTransitions m.(modelElements).
 
 Definition initialState (m: MooreModel) : option State :=
-    find (fun s => eqb "S0" (State_getName s)) (MooreMetamodel_allStates m).
+    find (fun s => eqb "S0" s.(name)) (MooreMetamodel_allStates m).
 
 
 Definition State_outTransitions (s: State) (m: MooreModel) : list Transition :=
@@ -30,7 +30,7 @@ Definition State_outTransitions (s: State) (m: MooreModel) : list Transition :=
         (MooreMetamodel_allTransitions m).
 
 Definition State_acceptTransition (s: State) (m: MooreModel) (i: string) : option Transition :=
-    find (fun t => eqb i (Transition_getInput t)) (State_outTransitions s m).
+    find (fun t => eqb i t.(input)) (State_outTransitions s m).
         
 Fixpoint executeFromState (m: MooreModel) (current: State) (remainingInput: list string) : list string :=
     match remainingInput with 
@@ -42,7 +42,7 @@ Fixpoint executeFromState (m: MooreModel) (current: State) (remainingInput: list
             | None => None
             end in
         match trgState with
-        | Some s => (State_getOutput s) :: (executeFromState m s is)
+        | Some s => s.(output) :: (executeFromState m s is)
         | None => nil
         end
     | _ => nil 
