transformations/Moore2Mealy/tests/sampleMoore.v
@@ -17,15 +17,15 @@ Open Scope string_scope.
 Definition InputModel : Model MooreMetamodel_Metamodel_Instance :=
 	(Build_Model MooreMetamodel_Metamodel_Instance
 		(
-		(Build_MooreMetamodel_Object TransitionClass (BuildTransition  "0")) :: 
-		(Build_MooreMetamodel_Object StateClass (BuildState  "S0" "1")) :: 
-		(Build_MooreMetamodel_Object StateClass (BuildState  "S1" "0")) :: 
-		(Build_MooreMetamodel_Object TransitionClass (BuildTransition  "1")) :: 
+		(Build_MooreMetamodel_Object Transition_K (BuildTransition  "0")) :: 
+		(Build_MooreMetamodel_Object State_K (BuildState  "S0" "1")) :: 
+		(Build_MooreMetamodel_Object State_K (BuildState  "S1" "0")) :: 
+		(Build_MooreMetamodel_Object Transition_K (BuildTransition  "1")) :: 
 		nil)
 		(
-		(Build_MooreMetamodel_Link TransitionSourceReference (BuildTransitionSource (BuildTransition  "0") (BuildState  "S1" "0"))) ::
-		(Build_MooreMetamodel_Link TransitionTargetReference (BuildTransitionTarget (BuildTransition  "0") (BuildState  "S0" "1"))) ::
-		(Build_MooreMetamodel_Link TransitionSourceReference (BuildTransitionSource (BuildTransition  "1") (BuildState  "S0" "1"))) ::
-		(Build_MooreMetamodel_Link TransitionTargetReference (BuildTransitionTarget (BuildTransition  "1") (BuildState  "S1" "0"))) ::
+		(Build_MooreMetamodel_Link TransitionSource_K (BuildTransitionSource (BuildTransition  "0") (BuildState  "S1" "0"))) ::
+		(Build_MooreMetamodel_Link TransitionTarget_K (BuildTransitionTarget (BuildTransition  "0") (BuildState  "S0" "1"))) ::
+		(Build_MooreMetamodel_Link TransitionSource_K (BuildTransitionSource (BuildTransition  "1") (BuildState  "S0" "1"))) ::
+		(Build_MooreMetamodel_Link TransitionTarget_K (BuildTransitionTarget (BuildTransition  "1") (BuildState  "S1" "0"))) ::
 		nil)
 	).
